Collect LogRel intro/inv, cleanup protect/cofine

LogRel/LR.v
@@ -21,29 +21,15 @@ Inductive Direction : Set :=
 Definition World := nat.
 Definition lev : World → nat := fun w => w.
 
-Definition PTRel := PTy -> S.Tm -> U.UTm -> Prop.
-Definition PCRel := PTy -> S.PCtx -> U.PCtx -> Prop.
+Definition PTRel := PTy → S.Tm → U.UTm → Prop.
+Definition PCRel := PTy → S.PCtx → U.PCtx → Prop.
 
 (* Intuitively: observing termination takes a step in addition to the actual evaluation steps *)
-Definition Observe (n : nat) (T : nat -> Prop) : Prop :=
-  match n with 
-      | 0 => False
-      | S n' => T n'
+Definition Observe (n : nat) (T : nat → Prop) : Prop :=
+  match n with
+    | 0 => False
+    | S n' => T n'
   end.
-
-Definition Obs (d : Direction) (w : World) (ts : S.Tm) (tu : U.UTm) :=
-  match d with
-    | dir_lt => Observe (lev w) (S.TerminatingN ts) → U.Terminating tu
-    | dir_gt => Observe (lev w) (U.TerminatingN tu)  → S.Terminating ts
-  end.
-
-Definition contrel'
-           (d : Direction) (w : World) (vr' : forall w' : World, w' ≤ w -> PTRel) : PCRel :=
- fun τ Cs Cu => forall w' (fw : w' ≤ w) ts tu, vr' w' fw τ ts tu -> Obs d w' (S.pctx_app ts Cs) (U.pctx_app tu Cu).
-
-Definition termrel'
-           (d : Direction) (w : World) (vr' : forall w' : World, w' ≤ w -> PTRel) : PTRel :=
-  fun τ ts tu => forall Cs Cu, S.ECtx Cs → U.ECtx Cu → contrel' d w vr' τ Cs Cu -> Obs d w (S.pctx_app ts Cs) (U.pctx_app tu Cu).
 
 Lemma lt_le {w w' w''} (fw : w' < w) (fw' : w'' ≤ w') : w'' < w.
 Proof.
@@ -79,130 +65,145 @@ Arguments prod_rel R₁ R₂ !ts !tu.
 Arguments sum_rel R₁ R₂ !ts !tu.
 Arguments arr_rel R₁ R₂ !ts !tu.
 
-Definition valrel'
-           (d : Direction) (w : World) (ind : forall w' : World, w' < w -> PTRel) : PTRel := 
-  fun τ ts tu =>
-    OfType τ ts tu ∧
-    let latervr : PTRel := fun τ ts tu => forall w' (fw : w' < w), ind w' fw τ ts tu in 
-    let laterlatervr : forall w' (fw : w' < w) w'' (fw' : w'' ≤ w'), PTRel := fun w' fw w'' fw' => ind w'' (lt_le fw fw') in 
-    let vrunit : S.Tm -> U.UTm -> Prop := fun ts tu => ts = S.unit ∧ tu = U.unit in
-    let vrbool : S.Tm -> U.UTm -> Prop := fun ts tu => (ts = S.true ∧ tu = U.true) ∨ (ts = S.false ∧ tu = U.false) in
-    let vrprod : PTy -> PTy -> S.Tm -> U.UTm -> Prop :=
-        fun τ₁ τ₂ =>
-          prod_rel (latervr τ₁) (latervr τ₂) in
-    let vrsum : PTy -> PTy -> S.Tm -> U.UTm -> Prop :=
-        fun τ₁ τ₂ =>
-          sum_rel (latervr τ₁) (latervr τ₂) in
-    let vrarr : PTy → PTy → S.Tm → U.UTm → Prop :=
-        fun τ₁ τ₂ ts tu =>
-          ∀ w' (fw : w' < w),
-            arr_rel
-              (ind w' fw τ₁)
-              (termrel' d w' (laterlatervr w' fw) τ₂)
-              ts tu
-    in
-    match τ with
-      | ptunit => vrunit ts tu
-      | ptbool => vrbool ts tu
-      | ptprod τ₁ τ₂ => vrprod τ₁ τ₂ ts tu
-      | ptsum τ₁ τ₂ => vrsum τ₁ τ₂ ts tu
-      | ptarr τ₁ τ₂ => vrarr τ₁ τ₂ ts tu
-      | pEmulDV n p => match n with
-                         | 0 => ts = S.unit ∧ p = imprecise
-                         | S n' => (ts = unkUVal (S n') ∧ p = imprecise) ∨
-                                   exists ts',
-                                     (ts = inUnit n ts' ∧ vrunit ts' tu) ∨
-                                     (ts = inBool n ts' ∧ vrbool ts' tu) ∨
-                                     (ts = inProd n ts' ∧ vrprod (pEmulDV n' p) (pEmulDV n' p) ts' tu) ∨
-                                     (ts = inSum n ts' ∧ vrsum (pEmulDV n' p) (pEmulDV n' p) ts' tu) ∨
-                                     (ts = inArr n ts' ∧ vrarr (pEmulDV n' p) (pEmulDV n' p) ts' tu)
-                       end
+Section LogicalRelation.
+
+  Variable (d: Direction).
+
+  Definition Obs (w : World) (ts : S.Tm) (tu : U.UTm) :=
+    match d with
+      | dir_lt => Observe (lev w) (S.TerminatingN ts) → U.Terminating tu
+      | dir_gt => Observe (lev w) (U.TerminatingN tu) → S.Terminating ts
     end.
 
-Definition valrel (d : Direction) (w : World) (τ : PTy)(t₁ : S.Tm) (t₂ : U.UTm) : Prop :=
-  Fix lt_wf (fun w => PTRel) (valrel' d) w τ t₁ t₂.
-Arguments valrel d w τ t₁ t₂ : simpl never.
+  Definition contrel' (w : World) (vr' : ∀ w' : World, w' ≤ w → PTRel) : PCRel :=
+   fun τ Cs Cu => ∀ w' (fw : w' ≤ w) ts tu, vr' w' fw τ ts tu → Obs w' (S.pctx_app ts Cs) (U.pctx_app tu Cu).
 
-Lemma valrel_def_funext {d} w (ind₁ ind₂ : forall w', w' < w → PTRel) :
-  (forall w' (fw : w' < w), ind₁ w' fw = ind₂ w' fw) →
-  valrel' d w ind₁ = valrel' d w ind₂.
-Proof.
-  intros.
-  enough (ind₁ = ind₂) as -> by auto.
-  extensionality w'.
-  extensionality fw.
-  trivial.
-Qed.
+  Definition termrel' (w : World) (vr' : ∀ w' : World, w' ≤ w → PTRel) : PTRel :=
+    fun τ ts tu => ∀ Cs Cu, S.ECtx Cs → U.ECtx Cu → contrel' w vr' τ Cs Cu → Obs w (S.pctx_app ts Cs) (U.pctx_app tu Cu).
 
-Lemma valrel_fixp {d} :
-  forall w, valrel d w = valrel' d w (fun w _ => valrel d w).
-Proof.
-  refine (Fix_eq lt_wf (fun w => PTRel) (valrel' d) valrel_def_funext).
-Qed.
+  Definition valrel' (w : World) (ind : ∀ w' : World, w' < w → PTRel) : PTRel :=
+    fun τ ts tu =>
+      OfType τ ts tu ∧
+      let latervr : PTRel := fun τ ts tu => ∀ w' (fw : w' < w), ind w' fw τ ts tu in
+      let laterlatervr : ∀ w' (fw : w' < w) w'' (fw' : w'' ≤ w'), PTRel := fun w' fw w'' fw' => ind w'' (lt_le fw fw') in
+      let vrunit : S.Tm → U.UTm → Prop := fun ts tu => ts = S.unit ∧ tu = U.unit in
+      let vrbool : S.Tm → U.UTm → Prop := fun ts tu => (ts = S.true ∧ tu = U.true) ∨ (ts = S.false ∧ tu = U.false) in
+      let vrprod : PTy → PTy → S.Tm → U.UTm → Prop :=
+          fun τ₁ τ₂ =>
+            prod_rel (latervr τ₁) (latervr τ₂) in
+      let vrsum : PTy → PTy → S.Tm → U.UTm → Prop :=
+          fun τ₁ τ₂ =>
+            sum_rel (latervr τ₁) (latervr τ₂) in
+      let vrarr : PTy → PTy → S.Tm → U.UTm → Prop :=
+          fun τ₁ τ₂ ts tu =>
+            ∀ w' (fw : w' < w),
+              arr_rel
+                (ind w' fw τ₁)
+                (termrel' w' (laterlatervr w' fw) τ₂)
+                ts tu
+      in
+      match τ with
+        | ptunit => vrunit ts tu
+        | ptbool => vrbool ts tu
+        | ptprod τ₁ τ₂ => vrprod τ₁ τ₂ ts tu
+        | ptsum τ₁ τ₂ => vrsum τ₁ τ₂ ts tu
+        | ptarr τ₁ τ₂ => vrarr τ₁ τ₂ ts tu
+        | pEmulDV n p => match n with
+                           | 0 => ts = S.unit ∧ p = imprecise
+                           | S n' => (ts = unkUVal (S n') ∧ p = imprecise) ∨
+                                     exists ts',
+                                       (ts = inUnit n ts' ∧ vrunit ts' tu) ∨
+                                       (ts = inBool n ts' ∧ vrbool ts' tu) ∨
+                                       (ts = inProd n ts' ∧ vrprod (pEmulDV n' p) (pEmulDV n' p) ts' tu) ∨
+                                       (ts = inSum n ts' ∧ vrsum (pEmulDV n' p) (pEmulDV n' p) ts' tu) ∨
+                                       (ts = inArr n ts' ∧ vrarr (pEmulDV n' p) (pEmulDV n' p) ts' tu)
+                         end
+      end.
 
-Definition contrel
-           (d : Direction) (w : World) : PCRel :=
-  contrel' d w (fun w fw => valrel d w).
+  Definition valrel (w : World) (τ : PTy)(t₁ : S.Tm) (t₂ : U.UTm) : Prop :=
+    Fix lt_wf (fun w => PTRel) valrel' w τ t₁ t₂.
 
-Definition termrel
-           (d : Direction) (w : World) : PTRel :=
-  termrel' d w (fun w fw => valrel d w).
+  Lemma valrel_def_funext w (ind₁ ind₂ : ∀ w', w' < w → PTRel) :
+    (∀ w' (fw : w' < w), ind₁ w' fw = ind₂ w' fw) →
+    valrel' w ind₁ = valrel' w ind₂.
+  Proof.
+    intros.
+    enough (ind₁ = ind₂) as -> by auto.
+    extensionality w'.
+    extensionality fw.
+    trivial.
+  Qed.
+
+  Lemma valrel_fixp : ∀ w, valrel w = valrel' w (fun w _ => valrel w).
+  Proof.
+    refine (Fix_eq lt_wf (fun w => PTRel) valrel' valrel_def_funext).
+  Qed.
+
+  Definition contrel (w : World) : PCRel :=
+    contrel' w (fun w fw => valrel w).
+
+  Definition termrel (w : World) : PTRel :=
+    termrel' w (fun w fw => valrel w).
+
+  Lemma termrel_fixp :
+    ∀ w, termrel w = termrel' w (fun w _ => valrel' w (fun w _ => valrel w)).
+  Proof.
+    unfold termrel.
+    intros w.
+    f_equal.
+    (* Should we avoid functional extensionality? *)
+    extensionality w'.
+    extensionality fw.
+    apply valrel_fixp.
+  Qed.
+
+  Definition envrel (w : World) (Γ : PEnv) (γs : Sub S.Tm) (γu : Sub U.UTm) : Prop :=
+    ∀ i τ, ⟪ i : τ p∈ Γ ⟫ → valrel w τ (γs i) (γu i).
+
+  Definition OpenLRN (n : nat) (Γ : PEnv) (ts : S.Tm) (tu : U.UTm) (τ : PTy) : Prop :=
+    ⟪ repEmulCtx Γ ⊢ ts : repEmul τ ⟫ ∧
+    ∀ w, lev w ≤ n → ∀ γs γu, envrel w Γ γs γu → termrel w τ (ts [ γs ]) (tu [ γu ]).
+
+  Definition OpenLR (Γ : PEnv) (ts : S.Tm) (tu : U.UTm) (τ : PTy) : Prop :=
+    ∀ n, OpenLRN n Γ ts tu τ.
+
+  Definition OpenLRCtxN (n : nat) (Cs : S.PCtx) (Cu : U.PCtx) (Γ' : PEnv) (τ' : PTy) (Γ : PEnv) (τ : PTy) : Prop :=
+    ⟪ ⊢ Cs : repEmulCtx Γ' , repEmul τ' → repEmulCtx Γ , repEmul τ ⟫ ∧
+    ∀ ts tu, OpenLRN n Γ' ts tu τ' -> OpenLRN n Γ (S.pctx_app ts Cs) (U.pctx_app tu Cu) τ.
+
+  Definition OpenLRCtx (Cs : S.PCtx) (Cu : U.PCtx) (Γ' : PEnv) (τ' : PTy) (Γ : PEnv) (τ : PTy) : Prop :=
+    ⟪ ⊢ Cs : repEmulCtx Γ' , repEmul τ' → repEmulCtx Γ' , repEmul τ ⟫ ∧
+    ∀ ts tu, OpenLR Γ' ts tu τ' → OpenLR Γ (S.pctx_app ts Cs) (U.pctx_app tu Cu) τ.
+
+End LogicalRelation.
 
 Arguments termrel d w τ t₁ t₂ : simpl never.
-
-Lemma termrel_fixp {d} :
-  forall w, termrel d w = termrel' d w (fun w _ => valrel' d w (fun w _ => valrel d w)).
-Proof.
-  unfold termrel. 
-  intros w.
-  f_equal.
-  (* Should we avoid functional extensionality? *)
-  extensionality w'.
-  extensionality fw.
-  apply valrel_fixp.
-Qed.
-
-Definition envrel (d : Direction) (w : World) (Γ : PEnv) (γs : Sub S.Tm) (γu : Sub U.UTm) : Prop :=
-  forall i τ, ⟪ i : τ p∈ Γ ⟫ → valrel d w τ (γs i) (γu i).
-
-Definition OpenLRN (d : Direction) (n : nat) (Γ : PEnv) (ts : S.Tm) (tu : U.UTm) (τ : PTy) : Prop :=
-  ⟪ repEmulCtx Γ ⊢ ts : repEmul τ ⟫ ∧
-  forall w, lev w ≤ n -> forall γs γu, envrel d w Γ γs γu -> termrel d w τ (ts [ γs ]) (tu [ γu ]).
+Arguments valrel d w τ t₁ t₂ : simpl never.
+Arguments valrel' d w ind !τ !t₁ !t₂ /.
 
 Notation "⟪ Γ ⊩ ts ⟦ d , n ⟧ tu : τ ⟫" := (OpenLRN d n Γ ts tu τ)
-  (at level 0, ts at level 98, 
+  (at level 0, ts at level 98,
    d at level 98, n at level 98,
    tu at level 98,
    Γ at level 98, τ at level 98,
    format "⟪ Γ ⊩  ts ⟦ d , n ⟧ tu  :  τ  ⟫").
 
-Definition OpenLR (d : Direction) (Γ : PEnv) (ts : S.Tm) (tu : U.UTm) (τ : PTy) : Prop :=
-  forall n, OpenLRN d n Γ ts tu τ.
-
 Notation "⟪ Γ ⊩ ts ⟦ d ⟧ tu : τ ⟫" := (OpenLR d Γ ts tu τ)
-  (at level 0, ts at level 98, 
+  (at level 0, ts at level 98,
    d at level 98, tu at level 98,
    Γ at level 98, τ at level 98,
    format "⟪ Γ ⊩  ts ⟦ d ⟧ tu  :  τ  ⟫").
 
-Definition OpenLRCtxN (d : Direction) (n : nat) (Cs : S.PCtx) (Cu : U.PCtx) (Γ' : PEnv) (τ' : PTy) (Γ : PEnv) (τ : PTy) : Prop :=
-  ⟪ ⊢ Cs : repEmulCtx Γ' , repEmul τ' → repEmulCtx Γ , repEmul τ ⟫ ∧
-  forall ts tu, OpenLRN d n Γ' ts tu τ' -> OpenLRN d n Γ (S.pctx_app ts Cs) (U.pctx_app tu Cu) τ.
-
 Notation "⟪ ⊩ Cs ⟦ d , n ⟧ Cu : Γ₀ , τ₀ → Γ , τ ⟫" := (OpenLRCtxN d n Cs Cu Γ₀ τ₀ Γ τ)
-  (at level 0, Cs at level 98, 
+  (at level 0, Cs at level 98,
    d at level 98, n at level 98,
    Cu at level 98,
    Γ₀ at level 98, τ₀ at level 98,
    Γ at level 98, τ at level 98,
    format "⟪  ⊩  Cs ⟦ d , n ⟧ Cu  :  Γ₀ ,  τ₀  →  Γ ,  τ  ⟫").
 
-Definition OpenLRCtx (d : Direction) (Cs : S.PCtx) (Cu : U.PCtx) (Γ' : PEnv) (τ' : PTy) (Γ : PEnv) (τ : PTy) : Prop :=
-  ⟪ ⊢ Cs : repEmulCtx Γ' , repEmul τ' → repEmulCtx Γ , repEmul τ ⟫ ∧
-  forall ts tu, OpenLR d Γ' ts tu τ' -> OpenLR d Γ (S.pctx_app ts Cs) (U.pctx_app tu Cu) τ.
-
 Notation "⟪ ⊩ Cs ⟦ d ⟧ Cu : Γ₀ , τ₀ → Γ , τ ⟫" := (OpenLRCtx d Cs Cu Γ₀ τ₀ Γ τ)
-  (at level 0, Cs at level 98, 
+  (at level 0, Cs at level 98,
    d at level 98, Cu at level 98,
    Γ₀ at level 98, τ₀ at level 98,
    Γ at level 98, τ at level 98,
