LogRel/LemmasIntro.v
@@ -1,0 +1,518 @@
+Require Stlc.SpecSyntax.
+Require Utlc.SpecSyntax.
+Require Import Stlc.SpecTyping.
+Require Import Stlc.LemmasTyping.
+Require Import Stlc.SpecEvaluation.
+Require Import Stlc.LemmasEvaluation.
+Require Import Utlc.SpecScoping.
+Require Import Utlc.LemmasScoping.
+Require Import Utlc.DecideEval.
+Require Import LogRel.PseudoType.
+Require Import LogRel.LemmasPseudoType.
+Require Import LogRel.LR.
+Require Import LogRel.LemmasLR.
+Require Import Omega.
+Require Import Db.Lemmas.
+Require Utlc.Fix.
+
+Local Ltac crushLRMatch :=
+  match goal with
+    | [ |- _ ∧ _ ] => split
+    | [ H : valrel _ _ ?τ ?ts ?tu   |- OfType ?τ ?ts ?tu ] => refine (valrel_implies_OfType H)
+    | [ H : valrel ?d _ ?τ ?ts ?tu  |- termrel ?d _ ?τ ?ts ?tu ] => apply valrel_in_termrel
+    | [ H : valrel ?d ?w ?τ ?ts ?tu |- valrel ?d ?w' ?τ ?ts ?tu ] => refine (valrel_mono _ H); omega
+    | [ |- valrel _ _ _ _ _] => rewrite -> valrel_fixp; unfold valrel'
+    | [ |- context[ lev ]] => unfold lev
+    | [ H : context[ lev ] |- _ ] => unfold lev in *
+  end.
+
+Local Ltac crush :=
+  repeat
+    (cbn;
+     destruct_conjs;
+     subst*;
+     repeat crushLRMatch;
+     crushOfType;
+     crushTyping;
+     repeat crushUtlcSyntaxMatchH;
+     trivial
+    ); try omega; eauto.
+
+Section ValueRelation.
+
+  (* Lambda abstraction *)
+  Lemma valrel_lambda {d τ' τ ts tu w} :
+    OfType (ptarr τ' τ) (S.abs (repEmul τ') ts) (U.abs tu) →
+    (∀ w' vs vu, w' < w → valrel d w' τ' vs vu → termrel d w' τ (ts [beta1 vs]) (tu [beta1 vu])) →
+    valrel d w (ptarr τ' τ) (S.abs (repEmul τ') ts) (U.abs tu).
+  Proof.
+    intros ot hyp; crush.
+    apply hyp; crush.
+  Qed.
+
+  (* Unit *)
+  Lemma valrel_unit {d w} :
+    valrel d w ptunit S.unit U.unit.
+  Proof. crush. Qed.
+
+  (* True *)
+  Lemma valrel_true {d w} :
+    valrel d w ptbool S.true U.true.
+  Proof. crush. Qed.
+
+  (* False *)
+  Lemma valrel_false {d w} :
+    valrel d w ptbool S.false U.false.
+  Proof. crush. Qed.
+
+  (* Pair *)
+  Lemma valrel_pair' {d w τ₁ τ₂ ts₁ ts₂ tu₁ tu₂} :
+    valrel d w τ₁ ts₁ tu₁ →
+    valrel d w τ₂ ts₂ tu₂ →
+    valrel d (S w) (ptprod τ₁ τ₂) (S.pair ts₁ ts₂) (U.pair tu₁ tu₂).
+  Proof. crush. Qed.
+
+  Lemma valrel_pair {d w τ₁ τ₂ ts₁ ts₂ tu₁ tu₂} :
+    valrel d w τ₁ ts₁ tu₁ →
+    valrel d w τ₂ ts₂ tu₂ →
+    valrel d w (ptprod τ₁ τ₂) (S.pair ts₁ ts₂) (U.pair tu₁ tu₂).
+  Proof. crush. Qed.
+
+  Lemma valrel_0_pair {d τ₁ τ₂ vs₁ vu₁ vs₂ vu₂} :
+    OfType τ₁ vs₁ vu₁ →
+    OfType τ₂ vs₂ vu₂ →
+    valrel d 0 (ptprod τ₁ τ₂) (S.pair vs₁ vs₂) (U.pair vu₁ vu₂).
+  Proof. crush. Qed.
+
+  (* Inl *)
+  Lemma valrel_0_inl {d τ₁ τ₂ vs vu} :
+    OfType τ₁ vs vu →
+    valrel d 0 (ptsum τ₁ τ₂) (S.inl vs) (U.inl vu).
+  Proof. crush. Qed.
+
+  Lemma valrel_inl {d w τ₁ τ₂ vs vu} :
+    valrel d w τ₁ vs vu →
+    valrel d w (ptsum τ₁ τ₂) (S.inl vs) (U.inl vu).
+  Proof. crush. Qed.
+
+  Lemma valrel_inl' {d w τ₁ τ₂ vs vu} :
+    valrel d w τ₁ vs vu →
+    valrel d (S w) (ptsum τ₁ τ₂) (S.inl vs) (U.inl vu).
+  Proof. crush. Qed.
+
+  (* Inr *)
+  Lemma valrel_0_inr {d τ₁ τ₂ vs vu} :
+    OfType τ₂ vs vu →
+    valrel d 0 (ptsum τ₁ τ₂) (S.inr vs) (U.inr vu).
+  Proof. crush. Qed.
+
+  Lemma valrel_inr {d w τ₁ τ₂ vs vu} :
+    valrel d w τ₂ vs vu →
+    valrel d w (ptsum τ₁ τ₂) (S.inr vs) (U.inr vu).
+  Proof. crush. Qed.
+
+  Lemma valrel_inr' {d w τ₁ τ₂ vs vu} :
+    valrel d w τ₂ vs vu →
+    valrel d (S w) (ptsum τ₁ τ₂) (S.inr vs) (U.inr vu).
+  Proof. crush. Qed.
+
+End ValueRelation.
+
+Ltac valrelIntro :=
+  match goal with
+    | |- valrel _ _ (ptarr ?τ _) (S.abs (repEmul ?τ) _) (U.abs _) => eapply valrel_lambda
+    | |- valrel _ _ ptunit S.unit U.unit => apply valrel_unit
+    | |- valrel _ _ ptbool S.true U.true => apply valrel_true
+    | |- valrel _ _ ptbool S.false U.false => apply valrel_false
+    | |- valrel _ ?w (ptprod _ _) (S.pair _ _) (U.pair _ _) =>
+      match w with
+        | O   => apply valrel_0_pair
+        | S _ => apply valrel_pair'
+        | _   => apply valrel_pair
+      end
+    | |- valrel _ ?w (ptsum _ _) (S.inl _) (U.inl _) =>
+      match w with
+        | O   => apply valrel_0_inl
+        | S _ => apply valrel_inl'
+        | _   => apply valrel_inl
+      end
+    | |- valrel _ ?w (ptsum _ _) (S.inr _) (U.inr _) =>
+      match w with
+        | O   => apply valrel_0_inr
+        | S _ => apply valrel_inr'
+        | _   => apply valrel_inr
+      end
+    | [ H : valrel ?d _ ?τ ?ts ?tu |- valrel ?d _ ?τ ?ts ?tu ] =>
+      refine (valrel_mono _ H); try omega
+  end.
+
+Section TermRelation.
+
+  (* Eval context *)
+  Lemma termrel_ectx {d w τ₁ τ₂ ts Cs tu Cu} (eCs : S.ECtx Cs) (eCu : U.ECtx Cu) :
+    termrel d w τ₁ ts tu →
+    (∀ w' (fw' : w' ≤ w) vs vu, valrel d w' τ₁ vs vu → termrel d w' τ₂ (S.pctx_app vs Cs) (U.pctx_app vu Cu)) →
+    termrel d w τ₂ (S.pctx_app ts Cs) (U.pctx_app tu Cu).
+  Proof.
+    intros tr cr Cs' Cu' eCs' eCu' cr'.
+    rewrite <- S.pctx_cat_app.
+    rewrite <- U.pctx_cat_app.
+    refine (tr (S.pctx_cat Cs Cs') (U.pctx_cat Cu Cu') _ _ _); eauto using S.ectx_cat, U.ectx_cat.
+    intros w' fw' vs vu vr.
+    destruct (valrel_implies_Value vr) as [vvs vvu].
+    rewrite -> S.pctx_cat_app.
+    rewrite -> U.pctx_cat_app.
+    refine (cr w' fw' vs vu vr Cs' Cu' eCs' eCu' _).
+    refine (contrel_mono fw' cr').
+  Qed.
+
+  Lemma termrel_ectx' {d w τ₁ τ₂ ts Cs tu ts' tu' Cu} :
+    termrel d w τ₁ ts tu →
+    (∀ w' (fw' : w' ≤ w) vs vu, valrel d w' τ₁ vs vu → termrel d w' τ₂ (S.pctx_app vs Cs) (U.pctx_app vu Cu)) →
+    ts' = S.pctx_app ts Cs →
+    tu' = U.pctx_app tu Cu →
+    S.ECtx Cs → U.ECtx Cu →
+    termrel d w τ₂ ts' tu'.
+  Proof.
+    intros; subst; eauto using termrel_ectx.
+  Qed.
+
+  (* Application *)
+  Lemma valrel_app {d w τ₁ τ₂ vs₁ vs₂ vu₁ vu₂} :
+    valrel d w (ptarr τ₁ τ₂) vs₁ vu₁ →
+    valrel d w τ₁ vs₂ vu₂ →
+    termrel d w τ₂ (S.app vs₁ vs₂) (U.app vu₁ vu₂).
+  Proof.
+    (* destruct assumptions *)
+    intros vr₁ vr₂.
+    rewrite -> valrel_fixp in vr₁.
+    destruct vr₁ as [ot hyp]; subst; cbn in hyp.
+    apply OfType_inversion_ptarr in ot.
+    destruct ot as (tsb & tub & eqs & equ & _); subst.
+    destruct (valrel_implies_Value vr₂) as [vvs₂ vvu₂].
+
+    (* beta-reduce *)
+    assert (es : S.eval (S.app (S.abs (repEmul τ₁) tsb) vs₂) (tsb [beta1 vs₂])) by
+        (refine (S.eval_ctx₀ S.phole _ I); refine (S.eval_beta vvs₂)).
+    assert (es1 : S.evaln (S.app (S.abs (repEmul τ₁) tsb) vs₂) (tsb [beta1 vs₂]) 1) by
+        (unfold S.evaln; eauto with eval; omega).
+    assert (eu : U.ctxeval (U.app (U.abs tub) vu₂) (tub [beta1 vu₂])) by
+        (refine (U.mkCtxEval U.phole _ _ I _); refine (U.eval_beta vvu₂)).
+    assert (eu1 : U.ctxevaln (U.app (U.abs tub) vu₂) (tub [beta1 vu₂]) 1) by
+        (unfold U.ctxevaln; eauto with eval).
+    destruct w; try apply termrel_zero.
+    refine (termrel_antired w es1 eu1 _ _ _); unfold lev in *; simpl; try omega.
+
+    (* use assumption for function body *)
+    eapply hyp; try omega; eauto using valrel_mono.
+  Qed.
+
+  Lemma termrel_app {d w τ₁ τ₂ ts₁ ts₂ tu₁ tu₂} :
+    termrel d w (ptarr τ₁ τ₂) ts₁ tu₁ →
+    (∀ w', w' ≤ w → termrel d w' τ₁ ts₂ tu₂) →
+    termrel d w τ₂ (S.app ts₁ ts₂) (U.app tu₁ tu₂).
+  Proof.
+    intros tr₁ tr₂.
+    change (S.app _ _) with (S.pctx_app ts₁ (S.papp₁ S.phole ts₂)).
+    change (U.app _ _) with (U.pctx_app tu₁ (U.papp₁ U.phole tu₂)).
+    refine (termrel_ectx _ _ tr₁ _); crush.
+    destruct (valrel_implies_Value H) as [vvs vvu].
+    change (S.app _ _) with (S.pctx_app ts₂ (S.papp₂ vs S.phole)).
+    change (U.app _ _) with (U.pctx_app tu₂ (U.papp₂ vu U.phole)).
+    refine (termrel_ectx _ _ (tr₂ w' fw')  _); crush.
+    refine (valrel_app _ H0); crush.
+  Qed.
+
+  Lemma termrel_ite {d w τ ts₁ ts₂ ts₃ tu₁ tu₂ tu₃} :
+    termrel d w ptbool ts₁ tu₁ →
+    (∀ w', w' ≤ w → termrel d w' τ ts₂ tu₂) →
+    (∀ w', w' ≤ w → termrel d w' τ ts₃ tu₃) →
+    termrel d w τ (S.ite ts₁ ts₂ ts₃) (U.ite tu₁ tu₂ tu₃).
+  Proof.
+    intros tr₁ tr₂ tr₃.
+
+    (* first evaluate ts₁ and tu₁ *)
+    change (S.ite _ _ _) with (S.pctx_app ts₁ (S.pite₁ S.phole ts₂ ts₃)).
+    change (U.ite _ _ _) with (U.pctx_app tu₁ (U.pite₁ U.phole tu₂ tu₃)).
+    refine (termrel_ectx _ _ tr₁ _); crush.
+
+    (* then evaluate the if-statement *)
+    rewrite -> valrel_fixp in H.
+    destruct H as [ot [[? ?]|[? ?]]]; subst; clear ot.
+    - assert (S.eval (S.ite S.true ts₂ ts₃) ts₂) by
+          (apply (S.eval_ctx₀ S.phole); try refine (S.eval_ite_true _ _); simpl; intuition).
+      assert (esn : S.evaln (S.ite S.true ts₂ ts₃) ts₂ 1) by (unfold S.evaln; eauto with eval).
+      assert (U.ctxeval (U.ite U.true tu₂ tu₃) tu₂) by
+          (apply (U.mkCtxEval U.phole); try refine (U.eval_ite_true _ _); simpl; intuition).
+      assert (eun : U.ctxevaln (U.ite U.true tu₂ tu₃) tu₂ 1) by (unfold U.ctxevaln; eauto with eval).
+      refine (termrel_antired w' esn eun _ _ _); crush.
+    - assert (S.eval (S.ite S.false ts₂ ts₃) ts₃) by
+          (apply (S.eval_ctx₀ S.phole); try refine (S.eval_ite_false _ _); simpl; intuition).
+      assert (esn : S.evaln (S.ite S.false ts₂ ts₃) ts₃ 1) by (unfold S.evaln; eauto with eval).
+      assert (U.ctxeval (U.ite U.false tu₂ tu₃) tu₃) by
+          (apply (U.mkCtxEval U.phole); try refine (U.eval_ite_false _ _); simpl; intuition).
+      assert (eun : U.ctxevaln (U.ite U.false tu₂ tu₃) tu₃ 1) by (unfold U.ctxevaln; eauto with eval).
+      refine (termrel_antired w' esn eun _ _ _); crush.
+  Qed.
+
+  (* Pair *)
+  Lemma termrel_pair {d w τ₁ τ₂ ts₁ ts₂ tu₁ tu₂} :
+    termrel d w τ₁ ts₁ tu₁ →
+    (∀ w', w' ≤ w → termrel d w' τ₂ ts₂ tu₂) →
+    termrel d w (ptprod τ₁ τ₂) (S.pair ts₁ ts₂) (U.pair tu₁ tu₂).
+  Proof.
+    intros tr₁ tr₂.
+    change (S.pair _ _) with (S.pctx_app ts₁ (S.ppair₁ S.phole ts₂)).
+    change (U.pair _ _) with (U.pctx_app tu₁ (U.ppair₁ U.phole tu₂)).
+    refine (termrel_ectx _ _ tr₁ _); crush.
+    destruct (valrel_implies_Value H) as [vvs₂ vvu₂].
+    change (S.pair _ _) with (S.pctx_app ts₂ (S.ppair₂ vs S.phole)).
+    change (U.pair _ _) with (U.pctx_app tu₂ (U.ppair₂ vu U.phole)).
+    refine (termrel_ectx _ _ (tr₂ w' fw')  _); crush.
+    eauto using valrel_in_termrel, valrel_mono, valrel_pair.
+  Qed.
+
+  (* Proj₁ *)
+  Lemma termrel_proj₁ {d w τ₁ τ₂ ts tu} :
+    termrel d w (ptprod τ₁ τ₂) ts tu →
+    termrel d w τ₁ (S.proj₁ ts) (U.proj₁ tu).
+  Proof.
+    intros tr.
+
+    (* first evaluate ts and tu *)
+    change (S.proj₁ _) with (S.pctx_app ts (S.pproj₁ S.phole)).
+    change (U.proj₁ _) with (U.pctx_app tu (U.pproj₁ U.phole)).
+    refine (termrel_ectx _ _ tr _); crush.
+
+    (* then evaluate the projection *)
+    rewrite -> valrel_fixp in H.
+    destruct H as [ot hyp]; subst; cbn in hyp.
+    apply OfType_inversion_ptprod in ot.
+    destruct ot as (vs₁ & vu₁ & vs₂ & vu₂ & ? & ? & ot₁ & ot₂); subst.
+    destruct (OfType_implies_Value ot₁) as [vvs₁ vvs₂].
+    destruct (OfType_implies_Value ot₂) as [vvu₁ vvu₂].
+    destruct hyp as [vr₁ vr₂].
+
+    assert (S.eval (S.proj₁ (S.pair vs₁ vs₂)) vs₁) by
+        (apply (S.eval_ctx₀ S.phole); try refine (S.eval_proj₁ _ _); simpl; intuition).
+    assert (esn : S.evaln (S.proj₁ (S.pair vs₁ vs₂)) vs₁ 1) by (unfold S.evaln; eauto with eval).
+    assert (U.ctxeval (U.proj₁ (U.pair vu₁ vu₂)) vu₁) by
+        (apply (U.mkCtxEval U.phole); try refine (U.eval_proj₁ _); simpl; intuition).
+    assert (eun : U.ctxevaln (U.proj₁ (U.pair vu₁ vu₂)) vu₁ 1) by (unfold U.ctxevaln; eauto with eval).
+    destruct w'; try apply termrel_zero.
+    refine (termrel_antired w' esn eun _ _ _); crush.
+
+    (* then conclude *)
+    apply valrel_in_termrel.
+    apply vr₁; intuition; omega.
+  Qed.
+
+  (* Proj₂ *)
+  Lemma termrel_proj₂ {d w τ₁ τ₂ ts tu} :
+    termrel d w (ptprod τ₁ τ₂) ts tu →
+    termrel d w τ₂ (S.proj₂ ts) (U.proj₂ tu).
+  Proof.
+    intros tr.
+
+    (* first reduce ts and tu *)
+    change (S.proj₂ _) with (S.pctx_app ts (S.pproj₂ S.phole)).
+    change (U.proj₂ _) with (U.pctx_app tu (U.pproj₂ U.phole)).
+    refine (termrel_ectx _ _ tr _); crush.
+
+    (* then evaluate the projection *)
+    rewrite -> valrel_fixp in H.
+    destruct H as [ot hyp]; subst; cbn in hyp.
+    apply OfType_inversion_ptprod in ot.
+    destruct ot as (vs₁ & vu₁ & vs₂ & vu₂ & ? & ? & ot₁ & ot₂); subst.
+    destruct (OfType_implies_Value ot₁) as [vvs₁ vvs₂].
+    destruct (OfType_implies_Value ot₂) as [vvu₁ vvu₂].
+    destruct hyp as [vr₁ vr₂].
+
+    assert (S.eval (S.proj₂ (S.pair vs₁ vs₂)) vs₂) by
+        (apply (S.eval_ctx₀ S.phole); try refine (S.eval_proj₂ _ _); simpl; intuition).
+    assert (esn : S.evaln (S.proj₂ (S.pair vs₁ vs₂)) vs₂ 1) by (unfold S.evaln; eauto with eval).
+    assert (U.ctxeval (U.proj₂ (U.pair vu₁ vu₂)) vu₂) by
+        (apply (U.mkCtxEval U.phole); try refine (U.eval_proj₂ _); simpl; intuition).
+    assert (eun : U.ctxevaln (U.proj₂ (U.pair vu₁ vu₂)) vu₂ 1)
+      by (unfold U.ctxevaln; eauto with eval).
+    destruct w'; try apply termrel_zero.
+    refine (termrel_antired w' esn eun _ _ _); crush.
+
+    apply valrel_in_termrel.
+    apply vr₂; crush.
+  Qed.
+
+  (* Inl *)
+  Lemma termrel_inl {d w τ₁ τ₂ ts tu} :
+    termrel d w τ₁ ts tu →
+    termrel d w (ptsum τ₁ τ₂) (S.inl ts) (U.inl tu).
+  Proof.
+    intros tr.
+    change (S.inl ts) with (S.pctx_app ts (S.pinl S.phole)).
+    change (U.inl tu) with (U.pctx_app tu (U.pinl U.phole)).
+    refine (termrel_ectx _ _ tr _); crush.
+    apply valrel_in_termrel; crush.
+  Qed.
+
+  (* Inr *)
+  Lemma termrel_inr {d w τ₁ τ₂ ts tu} :
+    termrel d w τ₂ ts tu →
+    termrel d w (ptsum τ₁ τ₂) (S.inr ts) (U.inr tu).
+  Proof.
+    intros tr.
+    change (S.inr ts) with (S.pctx_app ts (S.pinr S.phole)).
+    change (U.inr tu) with (U.pctx_app tu (U.pinr U.phole)).
+    refine (termrel_ectx _ _ tr _); crush.
+    apply valrel_in_termrel; crush.
+  Qed.
+
+  (* Caseof *)
+  Lemma termrel_caseof {d w τ τ₁ τ₂ ts₁ ts₂ ts₃ tu₁ tu₂ tu₃} :
+    termrel d w (ptsum τ₁ τ₂) ts₁ tu₁ →
+    (∀ w' vs₁ vu₁, w' < w → valrel d w' τ₁ vs₁ vu₁ → termrel d w' τ (ts₂ [beta1 vs₁]) (tu₂ [ beta1 vu₁])) →
+    (∀ w' vs₂ vu₂, w' < w → valrel d w' τ₂ vs₂ vu₂ → termrel d w' τ (ts₃ [beta1 vs₂]) (tu₃ [ beta1 vu₂])) →
+    termrel d w τ (S.caseof ts₁ ts₂ ts₃) (U.caseof tu₁ tu₂ tu₃).
+  Proof.
+    intros tr₁ tr₂ tr₃.
+
+    (* first evaluate ts₁ and tu₁ *)
+    change (S.caseof _ _ _) with (S.pctx_app ts₁ (S.pcaseof₁ S.phole ts₂ ts₃)).
+    change (U.caseof _ _ _) with (U.pctx_app tu₁ (U.pcaseof₁ U.phole tu₂ tu₃)).
+    refine (termrel_ectx _ _ tr₁ _); crush.
+
+    (* then evaluate the caseof *)
+    rewrite -> valrel_fixp in H.
+    destruct H as [ot hyp]; subst; cbn in hyp.
+    apply OfType_inversion_ptsum in ot.
+    destruct ot as (vs' & vu' & [(? & ? & ot)|[(? & ?)|[(? & ?)|(? & ? & ot)]]]);
+      subst; cbn in *; try contradiction;
+      destruct (OfType_implies_Value ot) as [vvs vvu]; clear ot.
+    - assert (S.eval (S.caseof (S.inl vs') ts₂ ts₃) (ts₂ [beta1 vs'])) by
+          (apply (S.eval_ctx₀ S.phole); try refine (S.eval_case_inl _); simpl; intuition).
+      assert (esn : S.evaln (S.caseof (S.inl vs') ts₂ ts₃) (ts₂ [beta1 vs']) 1) by (unfold S.evaln; eauto with eval).
+      assert (U.ctxeval (U.caseof (U.inl vu') tu₂ tu₃) (tu₂ [beta1 vu'])) by
+          (apply (U.mkCtxEval U.phole); try refine (U.eval_case_inl _ _); simpl; intuition).
+      assert (eun : U.ctxevaln (U.caseof (U.inl vu') tu₂ tu₃) (tu₂ [beta1 vu']) 1) by (unfold U.ctxevaln; eauto with eval).
+      destruct w'; try apply termrel_zero.
+      refine (termrel_antired w' esn eun _ _ _); crush.
+    - assert (S.eval (S.caseof (S.inr vs') ts₂ ts₃) (ts₃ [beta1 vs'])) by
+          (apply (S.eval_ctx₀ S.phole); try refine (S.eval_case_inr _); simpl; intuition).
+      assert (esn : S.evaln (S.caseof (S.inr vs') ts₂ ts₃) (ts₃ [beta1 vs']) 1) by (unfold S.evaln; eauto with eval).
+      assert (U.ctxeval (U.caseof (U.inr vu') tu₂ tu₃) (tu₃ [beta1 vu'])) by
+          (apply (U.mkCtxEval U.phole); try refine (U.eval_case_inr _ _); simpl; intuition).
+      assert (eun : U.ctxevaln (U.caseof (U.inr vu') tu₂ tu₃) (tu₃ [beta1 vu']) 1) by (unfold U.ctxevaln; eauto with eval).
+      destruct w'; try apply termrel_zero.
+      refine (termrel_antired w' esn eun _ _ _); crush.
+  Qed.
+
+  (* Seq *)
+  Lemma termrel_seq {d w τ ts₁ ts₂ tu₁ tu₂} :
+    termrel d w ptunit ts₁ tu₁ →
+    (∀ w', w' ≤ w → termrel d w' τ ts₂ tu₂) →
+    termrel d w τ (S.seq ts₁ ts₂) (U.seq tu₁ tu₂).
+  Proof.
+    intros tr₁ tr₂.
+
+    (* first evaluate ts₁ and tu₁ *)
+    change (S.seq _ _) with (S.pctx_app ts₁ (S.pseq₁ S.phole ts₂)).
+    change (U.seq _ _) with (U.pctx_app tu₁ (U.pseq₁ U.phole tu₂)).
+    refine (termrel_ectx _ _ tr₁ _); crush.
+
+    (* then reduce to ts₂ and tu₂ *)
+    rewrite -> valrel_fixp in H.
+    destruct H as [ot [eq₁ eq₂]]; subst.
+    assert (S.eval (S.seq S.unit ts₂) ts₂) by
+        (apply (S.eval_ctx₀ S.phole); try refine (S.eval_seq_next _); simpl; intuition).
+    assert (esn : S.evaln (S.seq S.unit ts₂) ts₂ 1) by (unfold S.evaln; eauto with eval).
+
+    (* assert (∀ Cu, U.ECtx Cu → U.eval (U.pctx_app (U.seq U.unit tu₂) Cu) (U.pctx_app tu₂ Cu)) by  *)
+    (*     (intros Cu eCu; apply (U.eval_ctx₀ Cu); try refine (U.eval_seq_next _); simpl; intuition). *)
+    (* assert (eun : ∀ Cu, U.ECtx Cu → U.evaln (U.pctx_app (U.seq U.unit tu₂) Cu) (U.pctx_app tu₂ Cu) 1) by eauto using U.evaln. *)
+
+    (* attempt at using evalMax instead of doing manual labor *)
+    pose (e := evalMax 2 (U.seq U.unit (var 0)) nil (idm UTm · tu₂) I).
+
+    refine (termrel_antired w' esn e _ _ _); try omega.
+
+    (* conclude *)
+    apply tr₂; intuition.
+  Qed.
+
+  (* Fixt *)
+  Lemma termrel_fix' {d w τ₁ τ₂ vs vu} :
+    valrel d w (ptarr (ptarr τ₁ τ₂) (ptarr τ₁ τ₂)) vs vu →
+    termrel d w (ptarr τ₁ τ₂) (S.fixt (repEmul τ₁) (repEmul τ₂) vs) (U.ufix₁ vu).
+  Proof.
+    (* well-founded induction on w *)
+    revert w vs vu.
+    refine (well_founded_ind lt_wf
+                             (fun w =>
+                                ∀ vs vu,
+                                  valrel d w (ptarr (ptarr τ₁ τ₂) (ptarr τ₁ τ₂)) vs vu →
+                                  termrel d w (ptarr τ₁ τ₂) (S.fixt (repEmul τ₁) (repEmul τ₂) vs) (U.ufix₁ vu)) _).
+    intros w indHyp vs vu.
+
+    (* destruct valrel assumption *)
+    intros vr.
+    rewrite -> valrel_fixp in vr.
+    destruct vr as [ot hyp]; cbn in hyp.
+    apply OfType_inversion_ptarr in ot.
+    destruct ot as (tsb & tub & ? & ? & ?); crush.
+
+    (* evaluate *)
+    assert (es : S.fixt (repEmul τ₁) (repEmul τ₂) (S.abs (repEmul (ptarr τ₁ τ₂)) tsb) --> tsb [beta1 (S.abs (repEmul τ₁) (S.app (S.fixt (repEmul τ₁) (repEmul τ₂) (S.abs (repEmul τ₁ ⇒ repEmul τ₂) tsb[wkm↑])) (S.var 0)))]) by (refine (eval_ctx₀ S.phole _ _); constructor).
+    assert (es1 : S.evaln (S.fixt (repEmul τ₁) (repEmul τ₂) (S.abs (repEmul (ptarr τ₁ τ₂)) tsb)) (tsb [beta1 (S.abs (repEmul τ₁) (S.app (S.fixt (repEmul τ₁) (repEmul τ₂) (S.abs (repEmul τ₁ ⇒ repEmul τ₂) tsb[wkm↑])) (S.var 0)))])  1) by
+        (unfold S.evaln; eauto with eval; omega).
+    assert (es2 : U.ctxevaln (U.ufix₁ (U.abs tub)) (tub[beta1 (U.abs (U.app (U.ufix₁ (U.abs tub[wkm↑])) (U.var 0)))]) 2) by
+        (eauto using U.ufix₁_evaln' with eval).
+    destruct w; try apply termrel_zero.
+    refine (termrel_antired w es1 es2 _ _ _); unfold lev in *; simpl; try omega.
+    clear es es1 es2.
+
+    (* use the assumption about tsb and tub we extracted from vr *)
+    refine (hyp w _ _ _ _); try omega.
+
+    (* prove valrel for values being substituted into tsb and tub *)
+    rewrite -> valrel_fixp.
+    unfold valrel'; cbn; split; intros.
+    - (* first the OfType relation *)
+      crush.
+    - (* prove the termrel of the body of the abstractions *)
+      refine (termrel_app (τ₁ := τ₁) (τ₂ := τ₂)_ _); crush.
+      change (abs (tub[wkm↑][wkm↑][(beta1 tu')↑↑])) with ((abs tub)[wkm][wkm][(beta1 tu')↑]).
+      change (S.abs _ _) with  ((S.abs (repEmul τ₁ ⇒ repEmul τ₂) tsb)[wkm][(beta1 ts')]).
+      rewrite <- apply_wkm_comm.
+      rewrite -> ?apply_wkm_beta1_cancel.
+      change (U.app _ _) with (U.ufix₁ (abs tub)).
+      (* the goal is now what we set out to prove initially but in a strictly
+             later world, so we can use the induction hypothesis from our
+             well-founded induction on worlds *)
+      refine (indHyp _ _ _ _ _); crush.
+      (* why do I need to call crush again? *)
+      eapply hyp; crush.
+  Qed.
+
+  Lemma termrel_fix {d w τ₁ τ₂ ts tu} :
+    termrel d w (ptarr (ptarr τ₁ τ₂) (ptarr τ₁ τ₂)) ts tu →
+    termrel d w (ptarr τ₁ τ₂) (S.fixt (repEmul τ₁) (repEmul τ₂) ts) (U.app U.ufix tu).
+  Proof.
+    intros tr.
+
+    (* first normalize ts and tu *)
+    change (S.fixt _ _ _) with (S.pctx_app ts (S.pfixt (repEmul τ₁) (repEmul τ₂) S.phole)).
+    change (U.app _ _) with (U.pctx_app tu (U.papp₂ U.ufix U.phole)).
+    refine (termrel_ectx _ _ tr _); crush.
+    destruct (valrel_implies_Value H) as [vvs vvu].
+
+    (* next, reduce (U.app U.ufix tu) by one step in the conclusion *)
+    assert (es1 : S.evaln (S.fixt (repEmul τ₁) (repEmul τ₂) vs) (S.fixt (repEmul τ₁) (repEmul τ₂) vs) 0) by
+        (unfold S.evaln; eauto with eval).
+    assert (es2 : U.ctxevaln (U.app U.ufix vu) (U.ufix₁ vu) 1)
+      by (unfold U.ctxevaln; eauto using U.ufix_eval₁' with eval).
+    refine (termrel_antired w' es1 es2 _ _ _); unfold lev in *; simpl; try omega.
+
+    (* then defer to valrel_fix *)
+    apply termrel_fix'; crush.
+  Qed.
+
+End TermRelation.
