LogRel/LemmasInversion.v
@@ -1,0 +1,91 @@
+Require Import Common.Common.
+Require Import LogRel.PseudoType.
+Require Import LogRel.LemmasPseudoType.
+Require Import LogRel.LR.
+Require Import LogRel.LemmasLR.
+Require Import Stlc.SpecSyntax.
+Require Import Stlc.SpecEvaluation.
+Require Import Stlc.LemmasEvaluation.
+Require Import Stlc.LemmasTyping.
+Require Import Stlc.SpecTyping.
+Require Import Utlc.SpecSyntax.
+Require Import Utlc.SpecEvaluation.
+Require Import Utlc.LemmasEvaluation.
+Require Import Utlc.Inst.
+
+Require Import Omega.
+Require Import Min.
+
+Section ValrelInversion.
+
+  Local Ltac crush :=
+    repeat
+      (simpl;
+       try assumption;
+       crushOfType;
+       repeat crushTyping;
+       repeat crushStlcSyntaxMatchH;
+       repeat crushUtlcSyntaxMatchH;
+       repeat crushUtlcScopingMatchH;
+       try subst;
+       destruct_conjs;
+       repeat match goal with
+                  [ |- _ ∧ _ ] => split
+              end;
+       eauto
+      ); try omega.
+
+  Lemma valrel_ptprod_inversion {d w τ₁ τ₂ vs vu} :
+    valrel d w (ptprod τ₁ τ₂) vs vu →
+    exists vs₁ vs₂ vu₁ vu₂,
+      (vs = S.pair vs₁ vs₂ ∧ vu = U.pair vu₁ vu₂ ∧
+       OfType τ₁ vs₁ vu₁ ∧
+       OfType τ₂ vs₂ vu₂ ∧
+       ∀ w', w' < w → valrel d w' τ₁ vs₁ vu₁ ∧ valrel d w' τ₂ vs₂ vu₂).
+  Proof.
+    intros vr.
+    destruct (valrel_implies_Value vr) as [vvs vvu].
+    destruct (OfType_inversion_ptprod (valrel_implies_OfType vr))
+      as (ts1' & tu1' & ts2' & tu2' & Hvs & Hvu & oft1 & oft2).
+    exists ts1', ts2', tu1', tu2'; do 4 (split; auto).
+    rewrite -> valrel_fixp in vr; subst vs vu.
+    unfold valrel' in vr; crush.
+  Qed.
+
+  Lemma valrel_ptsum_inversion {d w τ₁ τ₂ vs vu} :
+    valrel d w (ptsum τ₁ τ₂) vs vu →
+    exists vs' vu',
+      (vs = S.inl vs' ∧ vu = U.inl vu' ∧
+       OfType τ₁ vs' vu' ∧
+       ∀ w', w' < w → valrel d w' τ₁ vs' vu') ∨
+      (vs = S.inr vs' ∧ vu = U.inr vu' ∧
+       OfType τ₂ vs' vu' ∧
+       ∀ w', w' < w → valrel d w' τ₂ vs' vu').
+  Proof.
+    intros vr.
+    rewrite -> valrel_fixp in vr; destruct vr as [oft sumrel];
+    cbn in *; apply OfType_inversion_ptsum in oft;
+    destruct oft as (tsb & tub & Hvs); intuition; crush.
+    - exists tsb, tub; crush.
+    - exists tsb, tub; crush.
+  Qed.
+
+  Lemma valrel_ptarr_inversion {d w τ₁ τ₂ vs vu} :
+    valrel d w (ptarr τ₁ τ₂) vs vu →
+    ∃ tsb tub,
+      vs = S.abs (repEmul τ₁) tsb ∧ vu = U.abs tub ∧
+      ⟪ empty ▻ repEmul τ₁ ⊢ tsb : repEmul τ₂ ⟫ ∧
+      ∀ w' vs' vu',
+        w' < w → valrel d w' τ₁ vs' vu' →
+        termrel d w' τ₂ (tsb[beta1 vs']) (tub[beta1 vu']).
+  Proof.
+    intros vr.
+    destruct (valrel_implies_Value vr) as [vvs vvu].
+    destruct (OfType_inversion_ptarr (valrel_implies_OfType vr))
+      as (tsb & tub & Hvs & Hvu & wtsb).
+    exists tsb, tub; do 2 (split; auto).
+    rewrite -> valrel_fixp in vr; subst vs vu.
+    unfold valrel' in vr; unfold termrel; crush.
+  Qed.
+
+End ValrelInversion.
