LogRel/LemmasLR.v
@@ -331,34 +331,6 @@ Section ClosedLR.
       rewrite -> apply_wkm_beta1_cancel; intuition.
   Qed.
 
-  Lemma termrel_ectx {d w τ₁ τ₂ ts Cs tu Cu} (eCs : S.ECtx Cs) (eCu : U.ECtx Cu) :
-    termrel d w τ₁ ts tu →
-    (forall w' (fw' : w' ≤ w) vs vu, valrel d w' τ₁ vs vu → termrel d w' τ₂ (S.pctx_app vs Cs) (U.pctx_app vu Cu)) →
-    termrel d w τ₂ (S.pctx_app ts Cs) (U.pctx_app tu Cu).
-  Proof.
-    intros tr cr Cs' Cu' eCs' eCu' cr'.
-    rewrite <- S.pctx_cat_app.
-    rewrite <- U.pctx_cat_app.
-    refine (tr (S.pctx_cat Cs Cs') (U.pctx_cat Cu Cu') _ _ _); eauto using S.ectx_cat, U.ectx_cat.
-    intros w' fw' vs vu vr.
-    destruct (valrel_implies_Value vr) as [vvs vvu].
-    rewrite -> S.pctx_cat_app.
-    rewrite -> U.pctx_cat_app.
-    refine (cr w' fw' vs vu vr Cs' Cu' eCs' eCu' _).
-    refine (contrel_mono fw' cr').
-  Qed.
-
-  Lemma termrel_ectx' {d w τ₁ τ₂ ts Cs tu ts' tu' Cu} :
-    termrel d w τ₁ ts tu →
-    (forall w' (fw' : w' ≤ w) vs vu, valrel d w' τ₁ vs vu → termrel d w' τ₂ (S.pctx_app vs Cs) (U.pctx_app vu Cu)) →
-    ts' = S.pctx_app ts Cs →
-    tu' = U.pctx_app tu Cu →
-    S.ECtx Cs → U.ECtx Cu →
-    termrel d w τ₂ ts' tu'.
-  Proof.
-    intros; subst; eauto using termrel_ectx.
-  Qed.
-
   Lemma termrel_adequacy_lt {w m ts vs tu τ} :
     termrel dir_lt w τ ts tu →
     S.evaln ts vs m →
@@ -393,77 +365,6 @@ Section ClosedLR.
 
 End ClosedLR.
 
-Section ValrelInversion.
-  Local Ltac crush :=
-    repeat
-      (simpl;
-       try assumption;
-       crushOfType;
-       repeat crushTyping;
-       repeat crushStlcSyntaxMatchH;
-       repeat crushUtlcSyntaxMatchH;
-       repeat crushUtlcScopingMatchH;
-       try subst;
-       destruct_conjs;
-       repeat match goal with 
-                  [ |- _ ∧ _ ] => split
-              end;
-       eauto 
-      ); try omega.
-
-  Lemma valrel_ptprod_inversion {d w τ₁ τ₂ vs vu} :
-    valrel d w (ptprod τ₁ τ₂) vs vu →
-    exists vs₁ vs₂ vu₁ vu₂,
-      (vs = S.pair vs₁ vs₂ ∧ vu = U.pair vu₁ vu₂ ∧ 
-       OfType τ₁ vs₁ vu₁ ∧
-       OfType τ₂ vs₂ vu₂ ∧
-       ∀ w', w' < w → valrel d w' τ₁ vs₁ vu₁ ∧ valrel d w' τ₂ vs₂ vu₂).
-  Proof.
-    intros vr.
-    destruct (valrel_implies_Value vr) as [vvs vvu].
-    destruct (OfType_inversion_ptprod (valrel_implies_OfType vr))
-      as (ts1' & tu1' & ts2' & tu2' & Hvs & Hvu & oft1 & oft2).
-    exists ts1', ts2', tu1', tu2'; do 4 (split; auto).
-    rewrite -> valrel_fixp in vr; subst vs vu.
-    unfold valrel' in vr; crush.
-  Qed.
-
-  Lemma valrel_ptsum_inversion {d w τ₁ τ₂ vs vu} :
-    valrel d w (ptsum τ₁ τ₂) vs vu →
-    exists vs' vu',
-      (vs = S.inl vs' ∧ vu = U.inl vu' ∧ 
-       OfType τ₁ vs' vu' ∧
-       ∀ w', w' < w → valrel d w' τ₁ vs' vu') ∨
-      (vs = S.inr vs' ∧ vu = U.inr vu' ∧ 
-       OfType τ₂ vs' vu' ∧
-       ∀ w', w' < w → valrel d w' τ₂ vs' vu').
-  Proof.
-    intros vr.
-    rewrite -> valrel_fixp in vr; destruct vr as [oft sumrel];
-    cbn in *; apply OfType_inversion_ptsum in oft;
-    destruct oft as (tsb & tub & Hvs); intuition; crush.
-    - exists tsb, tub; crush.
-    - exists tsb, tub; crush.
-  Qed.
-
-  Lemma valrel_ptarr_inversion {d w τ₁ τ₂ vs vu} :
-    valrel d w (ptarr τ₁ τ₂) vs vu →
-    ∃ tsb tub,
-      vs = S.abs (repEmul τ₁) tsb ∧ vu = U.abs tub ∧
-      ⟪ empty ▻ repEmul τ₁ ⊢ tsb : repEmul τ₂ ⟫ ∧
-      ∀ w' vs' vu',
-        w' < w → valrel d w' τ₁ vs' vu' →
-        termrel d w' τ₂ (tsb[beta1 vs']) (tub[beta1 vu']).
-  Proof.
-    intros vr.
-    destruct (valrel_implies_Value vr) as [vvs vvu].
-    destruct (OfType_inversion_ptarr (valrel_implies_OfType vr))
-      as (tsb & tub & Hvs & Hvu & wtsb).
-    exists tsb, tub; do 2 (split; auto).
-    rewrite -> valrel_fixp in vr; subst vs vu.
-    unfold valrel' in vr; unfold termrel; crush.
-  Qed.
-End ValrelInversion.
       
 
 Section OpenLR.
